Lean/Egg/Core/Directions.lean
@@ -9,12 +9,12 @@ inductive Direction where
   deriving Inhabited, BEq, Hashable
 
 def Direction.description : Direction → String
-  | .forward  => "→"
-  | .backward => "←"
+  | forward  => "→"
+  | backward => "←"
 
 def Direction.merge : Direction → Direction → Direction
-  | .forward, .forward  | .backward, .backward => .forward
-  | .forward, .backward | .backward, .forward  => .backward
+  | forward, forward  | backward, backward => forward
+  | forward, backward | backward, forward  => backward
 
 -- IMPORTANT: The C interface to egg depends on the order of these constructors.
 inductive Directions where
@@ -22,27 +22,39 @@ inductive Directions where
   | forward
   | backward
   | both
+  deriving Inhabited, BEq, Hashable
+
+instance : Coe Direction Directions where
+  coe
+    | .forward  => .forward
+    | .backward => .backward
 
 namespace Directions
 
+def description : Directions → String
+  | none     => "∅"
+  | forward  => "→"
+  | backward => "←"
+  | both     => "↔"
+
 instance : ToString Directions where
   toString
-    | .none     => "none"
-    | .forward  => "forward"
-    | .backward => "backward"
-    | .both     => "both"
+    | none     => "none"
+    | forward  => "forward"
+    | backward => "backward"
+    | both     => "both"
 
 def contains : Directions → Direction → Bool
-  | .both, _ | .forward, .forward | .backward, .backward => true
-  | _, _                                                 => false
+  | both, _ | forward, .forward | backward, .backward => true
+  | _, _                                              => false
 
 -- The directions for which a given set is a superset of the other.
 def satisfyingSuperset (lhs rhs : RBTree α cmp) : Directions :=
   match rhs.subset lhs, lhs.subset rhs with
-  | false, false => .none
-  | false, true  => .backward
-  | true,  false => .forward
-  | true,  true  => .both
+  | false, false => none
+  | false, true  => backward
+  | true,  false => forward
+  | true,  true  => both
 
 -- The greatest lower bound of two given directions according to the lattice:
 --        both
@@ -51,7 +63,7 @@ def satisfyingSuperset (lhs rhs : RBTree α cmp) : Directions :=
 --      \     /
 --       none
 def meet : Directions → Directions → Directions
-  | .both, d | d, .both                                             => d
-  | .none, _ | _, .none | .backward, .forward | .forward, .backward => .none
-  | .forward, .forward                                              => .forward
-  | .backward, .backward                                            => .backward
+  | both, d | d, both                                         => d
+  | none, _ | _, none | backward, forward | forward, backward => none
+  | forward, forward                                          => forward
+  | backward, backward                                        => backward
