Lean/Egg/Core/Gen/TcSpecs.lean
@@ -6,20 +6,22 @@ open Lean Meta
 namespace Egg
 
 private partial def genSpecialization
-    (rw : Rewrite) (dir : Direction) (missing : MVarIdSet) (norm : Config.Normalization) :
-    MetaM (Option Rewrite) := do
-  let (rw, subst) ← rw.freshWithSubst (src := .tcSpec rw.src dir)
+    (rw : Rewrite) (dirs : Directions) (missing : MVarIdSet) (norm : Config.Normalization) :
+    MetaM (Rewrite × Bool) := do
+  let (rw, subst) ← rw.freshWithSubst (src := .tcSpec rw.src dirs)
   let mut missing := missing.map subst.expr.fwd.find!
-  let mut changed := true
-  while changed do
-    changed := false
+  let mut lastIterChanged := true
+  let mut everChanged := false
+  while lastIterChanged do
+    lastIterChanged := false
     for var in missing do
       if let some inst ← instanceForType? (← var.getType) then
         var.assign inst
         missing := missing.erase var
-        changed := true
+        lastIterChanged := true
+        everChanged := true
   let rw ← rw.instantiateMVars
-  return if rw.validDirs.contains dir then rw else none
+  return (rw, everChanged)
 where
   instanceForType? (type : Expr) : MetaM (Option Expr) := do
     if let some inst ← findLocalDeclWithType? type then
@@ -29,19 +31,25 @@ where
     else
       return none
 
-private def genTcSpecializationsForRw (rw : Rewrite) (norm : Config.Normalization) :
+private def genTcSpecializationsForRw (rw : Rewrite) (norm : Config.Normalization) (eager : Bool) :
     MetaM Rewrites := do
+  let mut specs : Rewrites := #[]
   let missingOnLhs := rw.mvars.rhs.tc.subtract rw.mvars.lhs.tc
   let missingOnRhs := rw.mvars.lhs.tc.subtract rw.mvars.rhs.tc
-  let mut specs : Rewrites := #[]
-  if !missingOnLhs.isEmpty then
-    if let some spec ← genSpecialization rw .forward missingOnLhs norm then
-    specs := specs.push spec
-  if !missingOnRhs.isEmpty then
-    if let some spec ← genSpecialization rw .backward missingOnRhs norm then
-    specs := specs.push spec
+  if let some fwd ← genDir .forward missingOnLhs then specs := specs.push fwd
+  if let some bwd ← genDir .backward missingOnRhs then specs := specs.push bwd
+  if eager then
+    let (spec, changed) ← genSpecialization rw .both (rw.mvars.lhs.tc.merge rw.mvars.rhs.tc) norm
+    if changed then specs := specs.push spec
   return specs
+where
+  genDir (dir : Direction) (missing : MVarIdSet) : MetaM (Option Rewrite) := do
+    unless !missing.isEmpty do return none
+    let (spec, _) ← genSpecialization rw dir missing norm
+    unless spec.validDirs.contains dir do return none
+    return spec
 
-def genTcSpecializations (targets : Rewrites) (norm : Config.Normalization) : MetaM Rewrites :=
+def genTcSpecializations (targets : Rewrites) (norm : Config.Normalization) (eager : Bool) :
+    MetaM Rewrites :=
   targets.foldlM (init := #[]) fun acc rw =>
-    return acc ++ (← genTcSpecializationsForRw rw norm)
+    return acc ++ (← genTcSpecializationsForRw rw norm eager)
