Lean/Egg/Tests/Eager TC Spec.lean
@@ -1,0 +1,19 @@
+import Egg
+
+class CommAdd (α) extends Add α where
+  comm : ∀ a b : α, a + b = b + a
+
+instance : CommAdd Nat where
+  comm := Nat.add_comm
+
+/-- error: egg failed to prove goal -/
+#guard_msgs in
+set_option egg.eagerTcSpec false in
+example (a : Nat) : a + b = b + a := by
+  letI := inferInstanceAs <| CommAdd Nat
+  egg [CommAdd.comm]
+
+set_option egg.eagerTcSpec true in
+example (a : Nat) : a + b = b + a := by
+  letI := inferInstanceAs <| CommAdd Nat
+  egg [CommAdd.comm]
